Grammar validate commutes

Validator/Hedge/Memoize/StateMemoize.lean
@@ -24,6 +24,10 @@ def StateMemoize.Grammar.derive.run {φ: Type} [DecidableEq φ] [Hashable φ]
   (state: memoizeState (φ × Ref n)) (G: Grammar n φ) (Φ: φ → α → Bool) (r: Regex (φ × Ref n)) (node: Node α): Regex (φ × Ref n) :=
   StateMemoize.run state (Grammar.Memoize.derive G Φ r node)
 
+def StateMemoize.Grammar.validate.run [DecidableEq φ] [Hashable φ]
+  (state: memoizeState (φ × Ref n)) (G: Grammar n φ) (Φ: φ → α → Bool) (nodes: Hedge α): Bool :=
+  StateMemoize.run state (Grammar.Memoize.validate G Φ nodes)
+
 lemma StateMemoize.Grammar.derive.run_unfold {φ: Type} [DecidableEq φ] [Hashable φ]
   (state: memoizeState (φ × Ref n)) (G: Grammar n φ) (Φ: φ → α → Bool) (r: Regex (φ × Ref n)) (node: Node α):
   (StateMemoize.Grammar.derive.run state G Φ r node) = StateMemoize.run state (Grammar.Memoize.derive G Φ r node) :=
@@ -47,3 +51,23 @@ theorem StateMemoize.Grammar.derive_commutes [DecidableEq φ] [Hashable φ]
   = Lang.derive (Grammar.Rule.denote G Φ r) node := by
   rw [StateMemoize.Grammar.derive.run_is_sound]
   rw [<- Grammar.Katydid.derive_commutes]
+
+lemma StateMemoize.Grammar.validate.run_unfold [DecidableEq φ] [Hashable φ]
+  (state: memoizeState (φ × Ref n)) (G: Grammar n φ) (Φ: φ → α → Bool) (nodes: Hedge α):
+  (StateMemoize.Grammar.validate.run state G Φ nodes) = StateMemoize.run state (Grammar.Memoize.validate G Φ nodes) :=
+  rfl
+
+theorem StateMemoize.validate.run_is_sound {φ: Type} {α: Type} [DecidableEq φ] [Hashable φ]
+  (state: memoizeState (φ × Ref n)) (G: Grammar n φ) (Φ: φ → α → Prop) [DecidableRel Φ] (nodes: Hedge α):
+  StateMemoize.Grammar.validate.run state G (decideRel Φ) nodes = Grammar.Katydid.validate G (decideRel Φ) nodes := by
+  rw [StateMemoize.Grammar.validate.run_unfold]
+  generalize StateMemoize.run state (Grammar.Memoize.validate G (decideRel Φ) nodes) = x
+  obtain ⟨b, hd⟩ := x
+  simp only
+  assumption
+
+theorem Regex.StateMemoize.validate_commutes {φ: Type} {α: Type} [DecidableEq φ] [Hashable φ]
+  (state: memoizeState (φ × Ref n)) (G: Grammar n φ) (Φ: φ → α → Prop) [DecidableRel Φ] (nodes: Hedge α):
+  StateMemoize.Grammar.validate.run state G (decideRel Φ) nodes = Grammar.denote G Φ nodes := by
+  rw [StateMemoize.validate.run_is_sound]
+  rw [<- Grammar.Katydid.validate_commutes]
